coq/NRA/Lang/NRA.v
@@ -14,6 +14,40 @@
  * limitations under the License.
  *)
 
+(** NRA is the Nested Relational Algebra. Although it is not directly
+in use in the compiler, replaced instead by NRAEnv, which extends it
+with a separate notion of environment, it is kept in the compiler as a
+reference. *)
+
+(** NRA is a small pure language without functions based on
+combinators (i.e., with no environment). Expressions in NRA take a
+single value as input. *)
+
+(** Summary:
+- Language: NRA (Nested Relational Algebra)
+- Based on: "Nested queries in object bases." Sophie Cluet and Guido
+  Moerkotte. Database Programming Languages (DBPL-4). Springer,
+  London, 1994. 226-242.
+- A more complete and recent treatment can be found in: "Building
+  Query Compilers", Chapter 7: An Algebra for Sets, Bags, and
+  Sequences. Guido Moerkotte, 2014.
+  http://pi3.informatik.uni-mannheim.de/~moer/querycompiler.pdf
+- translating to NRA: CAMP, cNRAEnv
+- translating from NRA: cNNRC, cNRAEnv *)
+
+(** Compared to the version from Cluet and Moerkotte:
+- We focus on a 'core' version of the algebra, suitable for semantics
+  and reasoning purposes. A number of important operators important
+  for optimization (e.g., GroupBy, Joins) are not considered, but can
+  be defined in terms of this 'core'.
+- We assume the existence of a global record containing global values
+  (in a database context those would be the input tables).
+- We add a [Default] operators which allows to test, and continue,
+  when a result is the empty bag.
+- We add two operators for matching against either values ([Either]
+  and [EitherConcat]).
+*)
+
 Section NRA.
   Require Import String.
   Require Import List.
@@ -22,266 +56,718 @@ Section NRA.
   Require Import Utils.
   Require Import CommonRuntime.
 
-  (** Nested Relational Algebra *)
-
-  (** By convention, "static" parameters come first, followed by
-     dependent operators. This allows for instanciation on those
-     parameters *)
-
   Context {fruntime:foreign_runtime}.
   
-  Inductive nra : Set :=
-  | AID : nra
-  | AConst : data -> nra
-  | ABinop : binary_op -> nra -> nra -> nra
-  | AUnop : unary_op -> nra -> nra
-  | AMap : nra -> nra -> nra
-  | AMapConcat : nra -> nra -> nra
-  | AProduct : nra -> nra -> nra
-  | ASelect : nra -> nra -> nra
-  | ADefault : nra -> nra -> nra
-  | AEither : nra -> nra -> nra
-  | AEitherConcat : nra -> nra -> nra
-  | AApp : nra -> nra -> nra
-  | AGetConstant : string -> nra
-  .
+  (** * Abstract Syntax *)
 
-  Global Instance nra_eqdec : EqDec nra eq.
-  Proof.
-    change (forall x y : nra,  {x = y} + {x <> y}).
-    decide equality;
-    try solve [apply binary_op_eqdec | apply unary_op_eqdec | apply data_eqdec | apply string_eqdec].
-  Qed.
-
-  (** NRA Semantics *)
-
-  Context (h:list(string*string)).
-  Section Semantics.
-    Context (constant_env:list (string*data)).
+  Section Syntax.
   
-    Fixpoint nra_eval (op:nra) (x:data) : option data :=
-      match op with
-      | AID => Some x
-      | AConst rd => Some (normalize_data h rd)
-      | ABinop bop op1 op2 =>
-        olift2 (fun d1 d2 => binary_op_eval h bop d1 d2) (nra_eval op1 x) (nra_eval op2 x)
-      | AUnop uop op1 =>
-        olift (fun d1 => unary_op_eval h uop d1) (nra_eval op1 x)
-      | AMap op1 op2 =>
-        let aux_map d :=
-            lift_oncoll (fun c1 => lift dcoll (rmap (nra_eval op1) c1)) d
-        in olift aux_map (nra_eval op2 x)
-      | AMapConcat op1 op2 =>
-        let aux_mapconcat d :=
-            lift_oncoll (fun c1 => lift dcoll (rmap_concat (nra_eval op1) c1)) d
-        in olift aux_mapconcat (nra_eval op2 x)
-      | AProduct op1 op2 =>
-        (* Note: (fun y => nra_eval op2 x) does not depend on input,
-           but we still use a nested loop and delay op2 evaluation so it does not
-           fail in case the op1 operand is an empty collection -- this makes sure
-           to align the semantics with the NNRC version. - Jerome *)
-        let aux_product d :=
-            lift_oncoll (fun c1 => lift dcoll (rmap_concat (fun _ => nra_eval op2 x) c1)) d
-        in olift aux_product (nra_eval op1 x)
-      | ASelect op1 op2 =>
-        let pred x' :=
-            match nra_eval op1 x' with
+  (** By convention, "static" parameters come first, followed by
+     so-called dependent operators. This allows for easy instanciation
+     on those parameters *)
+
+    Inductive nra : Set :=
+    | NRAGetConstant : string -> nra
+    | NRAID : nra
+    | NRAConst : data -> nra
+    | NRABinop : binary_op -> nra -> nra -> nra
+    | NRAUnop : unary_op -> nra -> nra
+    | NRAMap : nra -> nra -> nra
+    | NRAMapProduct : nra -> nra -> nra
+    | NRAProduct : nra -> nra -> nra
+    | NRASelect : nra -> nra -> nra
+    | NRADefault : nra -> nra -> nra
+    | NRAEither : nra -> nra -> nra
+    | NRAEitherConcat : nra -> nra -> nra
+    | NRAApp : nra -> nra -> nra.
+
+    (** Equality between two NRA expressions is decidable. *)
+  
+    Global Instance nra_eqdec : EqDec nra eq.
+    Proof.
+      change (forall x y : nra,  {x = y} + {x <> y}).
+      decide equality;
+        try solve [apply binary_op_eqdec | apply unary_op_eqdec | apply data_eqdec | apply string_eqdec].
+    Qed.
+
+  End Syntax.
+
+  (** * Semantics *)
+  
+  Section Semantics.
+    (** Part of the context is fixed for the rest of the development:
+- [h] is the brand relation
+- [constant_env] is the global environment *)
+
+    Context (h:list(string*string)).
+    Context (constant_env:list (string*data)).
+
+    Section Denotation.
+      Inductive rec_concat_sem: data -> data -> data -> Prop :=
+      | sem_rec_concat:
+          forall r1 r2,
+            rec_concat_sem (drec r1) (drec r2)
+                           (drec (rec_concat_sort r1 r2)).
+
+      Lemma orecconcat_correct : forall d d1 d2,
+          orecconcat d d1 = Some d2 ->
+          rec_concat_sem d d1 d2.
+      Proof.
+        intros.
+        destruct d; destruct d1; simpl in *; try congruence.
+        inversion H; econstructor; reflexivity.
+      Qed.
+
+      Lemma orecconcat_complete : forall d d1 d2,
+          rec_concat_sem d d1 d2 ->
+          orecconcat d d1 = Some d2.
+      Proof.
+        intros.
+        inversion H; subst.
+        reflexivity.
+      Qed.
+
+      Lemma orecconcat_correct_and_complete : forall d d1 d2,
+          orecconcat d d1 = Some d2 <->
+          rec_concat_sem d d1 d2.
+      Proof.
+        split.
+        apply orecconcat_correct.
+        apply orecconcat_complete.
+      Qed.
+        
+      Inductive map_concat_sem: data -> list data -> list data -> Prop :=
+      | sem_map_concat_empty : forall d,
+          map_concat_sem d nil nil                     (**r   d χ⊕ {} ⇓ {} *)
+      | sem_map_concat_cons : forall d d1 d2 c1 c2,
+          rec_concat_sem d d1 d2 ->                    (**r   d ⊕ d₁ ⇓ d₂ *)
+          map_concat_sem d c1 c2 ->                    (**r ∧ d χ⊕ {c₁} ⇓ {c₂} *)
+          map_concat_sem d (d1::c1) (d2::c2).          (**r ⇒ d χ⊕ {d₁::c₁} ⇓ {d₂::c₂} *)
+
+      Lemma omap_concat_correct d c1 c2:
+        omap_concat d c1 = Some c2 ->
+        map_concat_sem d c1 c2.
+      Proof.
+        unfold omap_concat.
+        revert c2.
+        induction c1; simpl; intros.
+        - inversion H; subst; econstructor.
+        - case_eq (orecconcat d a); intros; rewrite H0 in *; [|congruence].
+          rewrite orecconcat_correct_and_complete in H0.
+          unfold lift in H.
+          case_eq (rmap (fun x : data => orecconcat d x) c1); intros;
+            rewrite H1 in *; clear H1; [|congruence].
+          inversion H; subst; clear H.
+          specialize (IHc1 l eq_refl).
+          econstructor; eauto.
+      Qed.
+      
+      Lemma omap_concat_complete d c1 c2:
+        map_concat_sem d c1 c2 ->
+        omap_concat d c1 = Some c2.
+      Proof.
+        unfold omap_concat.
+        revert c2.
+        induction c1; simpl; intros.
+        - inversion H; reflexivity.
+        - inversion H; subst; simpl in *.
+          rewrite <- orecconcat_correct_and_complete in H3.
+          rewrite H3; simpl.
+          unfold lift.
+          rewrite (IHc1 c3 H5); reflexivity.
+      Qed.
+      
+      Lemma omap_concat_correct_and_complete d c1 c2:
+        omap_concat d c1 = Some c2 <->
+        map_concat_sem d c1 c2.
+      Proof.
+        split.
+        apply omap_concat_correct.
+        apply omap_concat_complete.
+      Qed.
+
+      Inductive product_sem: list data -> list data -> list data -> Prop :=
+      | sem_product_empty : forall c,
+          product_sem nil c nil                   (**r   [{c} × {} ⇓ {}] *)
+      | sem_product_cons : forall d1 c1 c2 c3 c4,
+          map_concat_sem d1 c2 c3 ->              (**r ∧ d1 χ× {c₂} ⇓ {c₃} *)
+          product_sem c1 c2 c4 ->                 (**r ∧ [{c₁} × {c₂} ⇓ {c₄}] *)
+          product_sem (d1::c1) c2 (c3 ++ c4).     (**r ⇒ [{d₁::c₁} × {c₂} ⇓ {c₃}∪{c₄}] *)
+
+      Lemma rproduct_correct c1 c2 c3:
+        rproduct c1 c2 = Some c3 ->
+        product_sem c1 c2 c3.
+      Proof.
+        unfold rproduct.
+        revert c2 c3.
+        induction c1; simpl; intros.
+        - inversion H; econstructor.
+        - case_eq (omap_concat a c2); intros; rewrite H0 in *; [|congruence].
+          unfold lift in H.
+          case_eq (oflat_map (fun x : data => omap_concat x c2) c1);
+            intros; rewrite H1 in *; [|congruence].
+          inversion H; subst; clear H.
+          specialize (IHc1 c2 l0 H1).
+          econstructor;[|assumption].
+          rewrite omap_concat_correct_and_complete in H0;assumption.
+      Qed.
+
+      Lemma rproduct_complete c1 c2 c3:
+        product_sem c1 c2 c3 ->
+        rproduct c1 c2 = Some c3.
+      Proof.
+        unfold rproduct.
+        revert c2 c3.
+        induction c1; simpl; intros.
+        - inversion H; subst; reflexivity.
+        - inversion H; subst.
+          rewrite <- omap_concat_correct_and_complete in H2.
+          rewrite H2.
+          unfold lift; rewrite (IHc1 c2 c6 H5).
+          reflexivity.
+      Qed.
+
+      Lemma rproduct_correct_and_complete c1 c2 c3:
+        rproduct c1 c2 = Some c3 <->
+        product_sem c1 c2 c3.
+      Proof.
+        split.
+        apply rproduct_correct.
+        apply rproduct_complete.
+      Qed.
+
+      Inductive nra_sem: nra -> data -> data -> Prop :=
+      | sem_NRAGetConstant : forall v din d,
+          edot constant_env v = Some d ->             (**r   [Γc(v) = d] *)
+          nra_sem (NRAGetConstant v) din d            (**r ⇒ [Γc ; Γ ⊢〚$$v〛⇓ d] *)
+      | sem_NRAID : forall din,
+          nra_sem NRAID din din
+      | sem_NRAConst : forall din d d1,
+          normalize_data h d = d1 ->
+          nra_sem (NRAConst d) din d1
+      | sem_NRABinop : forall bop e1 e2 din d1 d2 d3,
+          nra_sem e1 din d1 ->
+          nra_sem e2 din d2 ->
+          binary_op_eval h bop d1 d2 = Some d3 ->
+          nra_sem (NRABinop bop e1 e2) din d3
+      | sem_NRAUnop : forall uop e din d1 d2,
+          nra_sem e din d1 ->
+          unary_op_eval h uop d1 = Some d2 ->
+          nra_sem (NRAUnop uop e) din d2
+      | sem_NRAMap : forall e1 e2 din c1 c2,
+          nra_sem e1 din (dcoll c1) ->
+          nra_sem_map e2 c1 c2 ->
+          nra_sem (NRAMap e2 e1) din (dcoll c2)
+      | sem_NRAMapProduct : forall e1 e2 din c1 c2,
+          nra_sem e1 din (dcoll c1) ->
+          nra_sem_map_product e2 c1 c2 ->
+          nra_sem (NRAMapProduct e2 e1) din (dcoll c2)
+      | sem_NRAProduct : forall e1 e2 din c1 c2 c3,
+          nra_sem e1 din (dcoll c1) ->
+          nra_sem e2 din (dcoll c2) ->
+          product_sem c1 c2 c3 ->
+          nra_sem (NRAProduct e1 e2) din (dcoll c3)
+      | sem_NRASelect : forall e1 e2 din c1 c2,
+          nra_sem e1 din (dcoll c1) ->
+          nra_sem_select e2 c1 c2 ->
+          nra_sem (NRASelect e2 e1) din (dcoll c2)
+      | sem_NRADefault_empty : forall e1 e2 din d2,
+          nra_sem e1 din (dcoll nil) ->
+          nra_sem e2 din d2 ->
+          nra_sem (NRADefault e1 e2) din d2
+      | sem_NRADefault_not_empty : forall e1 e2 din d1,
+          d1 <> dcoll nil ->
+          nra_sem e1 din d1 ->
+          nra_sem (NRADefault e1 e2) din d1
+      | sem_NRAEither_left : forall e1 e2 d1 d3,
+          nra_sem e1 d1 d3 ->
+          nra_sem (NRAEither e1 e2) (dleft d1) d3
+      | sem_NRAEither_right : forall e1 e2 d1 d3,
+          nra_sem e2 d1 d3 ->
+          nra_sem (NRAEither e1 e2) (dright d1) d3
+      | sem_NRAEitherConcat_left : forall e1 e2 d r1 r2,
+          nra_sem e1 d (dleft (drec r1)) ->
+          nra_sem e2 d (drec r2) ->
+          nra_sem (NRAEitherConcat e1 e2) d (dleft (drec (rec_concat_sort r1 r2)))
+      | sem_NRAEitherConcat_right : forall e1 e2 d r1 r2,
+          nra_sem e1 d (dright (drec r1)) ->
+          nra_sem e2 d (drec r2) ->
+          nra_sem (NRAEitherConcat e1 e2) d (dright (drec (rec_concat_sort r1 r2)))
+      | sem_NRAApp : forall e1 e2 din d1 d2,
+          nra_sem e1 din d1 ->
+          nra_sem e2 d1 d2 ->
+          nra_sem (NRAApp e2 e1) din d2
+      with nra_sem_map: nra -> list data -> list data -> Prop :=
+      | sem_NRAMMap_empty : forall e,
+          nra_sem_map e nil nil                       (**r   [Γc ; {} ⊢〚e〛χ ⇓ {}] *)
+      | sem_NRAMap_cons : forall e d1 c1 d2 c2,
+          nra_sem e d1 d2 ->                          (**r   [Γc ; d₁ ⊢〚e〛⇓ d₂]  *)
+          nra_sem_map e c1 c2 ->                      (**r ∧ [Γc ; {c₁} ⊢〚e〛χ ⇓ {c₂}] *)
+          nra_sem_map e (d1::c1) (d2::c2)             (**r ⇒ [Γc ; {d₁::c₁} ⊢〚e〛χ ⇓ {d₂::c₂}] *)
+      with nra_sem_map_product: nra -> list data -> list data -> Prop :=
+      | sem_NRAMapProduct_empty : forall e,
+          nra_sem_map_product e nil nil               (**r   [Γc ; {} ⊢〚e〛⋈ᵈ ⇓ {}] *)
+      | sem_NRAMapProduct_cons : forall e d1 c1 c2 c3 c4,
+          nra_sem e d1 (dcoll c3) ->                  (**r   [Γc ; d₁ ⊢〚e〛⋈ᵈ ⇓ {c₃}]  *)
+          map_concat_sem d1 c3 c4 ->                  (**r ∧ d₁ χ⊕ c₃ ⇓ c₄ *)
+          nra_sem_map_product e c1 c2 ->              (**r ∧ [Γc ; {c₁} ⊢〚e〛⋈ᵈ ⇓ {c₂}] *)
+          nra_sem_map_product e (d1::c1) (c4 ++ c2)   (**r ⇒ [Γc ; {d₁::c₁} ⊢〚e〛⋈ᵈ ⇓ {c₄}∪{c₂}] *)
+      with nra_sem_select: nra -> list data -> list data -> Prop :=
+      | sem_NRASelect_empty : forall e,
+          nra_sem_select e nil nil                    (**r   [Γc ; {} ⊢〚e〛σ ⇓ {}] *)
+      | sem_NRASelect_true : forall e d1 c1 c2,
+          nra_sem e d1 (dbool true) ->                (**r   [Γc ; d₁ ⊢〚e〛σ ⇓ true]  *)
+          nra_sem_select e c1 c2 ->                   (**r ∧ [Γc ; {c₁} ⊢〚e〛σ ⇓ {c₂}] *)
+          nra_sem_select e (d1::c1) (d1::c2)          (**r ⇒ [Γc ; {d₁::c₁} ⊢〚e〛σ ⇓ {d₁::c₂}] *)
+      | sem_NRASelect_false : forall e d1 c1 c2,
+          nra_sem e d1 (dbool false) ->               (**r   [Γc ; d₁ ⊢〚e〛σ ⇓ false]  *)
+          nra_sem_select e c1 c2 ->                   (**r ∧ [Γc ; {c₁} ⊢〚e〛σ ⇓ {c₂}] *)
+          nra_sem_select e (d1::c1) c2                (**r ⇒ [Γc ; {d₁::c₁} ⊢〚e〛σ ⇓ {c₂}] *)
+      .
+
+    (** Note that there is (resp is not) a call to [nra_sem] inside
+    the [nra_sem_map] (resp [nra_sem_map_concat]) judgment, which
+    shows the distinction between so-called dependent product and a
+    regular Cartesian product. *)
+
+    End Denotation.
+
+    Section Evaluation.
+      
+      Fixpoint nra_eval (e:nra) (din:data) : option data :=
+        match e with
+        | NRAGetConstant s =>
+          edot constant_env s
+        | NRAID =>
+          Some din
+        | NRAConst d =>
+          Some (normalize_data h d)
+        | NRABinop bop e1 e2 =>
+          olift2
+            (fun d1 d2 => binary_op_eval h bop d1 d2)
+            (nra_eval e1 din) (nra_eval e2 din)
+        | NRAUnop uop e =>
+          olift (fun d1 => unary_op_eval h uop d1) (nra_eval e din)
+        | NRAMap e2 e1 =>
+          let aux_map c1 :=
+              lift_oncoll (fun d1 => lift dcoll (rmap (nra_eval e2) d1)) c1
+          in olift aux_map (nra_eval e1 din)
+        | NRAMapProduct e2 e1 =>
+          let aux_mapconcat c1 :=
+              lift_oncoll (fun d1 => lift dcoll (rmap_product (nra_eval e2) d1)) c1
+          in olift aux_mapconcat (nra_eval e1 din)
+        | NRAProduct e1 e2 =>
+          (* Note: (fun y => nra_eval op2 x) does not depend on input,
+             but we still use a nested loop and delay op2 evaluation
+             so it does not fail in case the op1 operand is an empty
+             collection -- this makes sure to align the semantics with
+             the NNRC version. - Jerome *)
+          let aux_product d :=
+              lift_oncoll (fun c1 => lift dcoll (rmap_product (fun _ => nra_eval e2 din) c1)) d
+          in olift aux_product (nra_eval e1 din)
+        | NRASelect e2 e1 =>
+          let pred d1 :=
+              match nra_eval e2 d1 with
               | Some (dbool b) => Some b
               | _ => None
-            end
-        in
-        let aux_select d :=
-            lift_oncoll (fun c1 => lift dcoll (lift_filter pred c1)) d
-        in
-        olift aux_select (nra_eval op2 x)
-      | ADefault op1 op2 =>
-        olift (fun d1 => match d1 with
-                           | dcoll nil => nra_eval op2 x
-                           | _ => Some d1
-                         end) (nra_eval op1 x)
-      | AEither opl opr =>
-        match x with
-          | dleft dl => nra_eval opl dl
-          | dright dr => nra_eval opr dr
+              end
+          in
+          let aux_select c1 :=
+              lift_oncoll (fun d1 => lift dcoll (lift_filter pred d1)) c1
+          in
+          olift aux_select (nra_eval e1 din)
+        | NRADefault e1 e2 =>
+          olift (fun d1 =>
+                   match d1 with
+                   | dcoll nil => nra_eval e2 din
+                   | _ => Some d1
+                   end)
+                (nra_eval e1 din)
+        | NRAEither e1 e2 =>
+          match din with
+          | dleft d1 => nra_eval e1 d1
+          | dright d2 => nra_eval e2 d2
           | _ => None
-        end
-      | AEitherConcat op1 op2 =>
-        match nra_eval op1 x, nra_eval op2 x with
+          end
+        | NRAEitherConcat e1 e2 =>
+          match nra_eval e1 din, nra_eval e2 din with
           | Some (dleft (drec l)), Some (drec t)  =>
             Some (dleft (drec (rec_concat_sort l t)))
           | Some (dright (drec r)), Some (drec t)  =>
             Some (dright (drec (rec_concat_sort r t)))
           | _, _ => None
-        end
-      | AApp op1 op2 =>
-        olift (fun d => (nra_eval op1 d)) (nra_eval op2 x)
-      | AGetConstant s => edot constant_env s
-    end.
+          end
+        | NRAApp e2 e1 =>
+          olift (fun d1 => (nra_eval e2 d1)) (nra_eval e1 din)
+        end.
+    End Evaluation.
 
-    Lemma data_normalized_orecconcat {x y z}:
-      orecconcat x y = Some z ->
-      data_normalized h x -> data_normalized h y ->
-      data_normalized h z.
-    Proof.
-      destruct x; simpl; try discriminate.
-      destruct y; simpl; try discriminate.
-      inversion 1; subst.
-      apply data_normalized_rec_concat_sort; trivial.
-    Qed.
+    Section EvalCorrect.
+      Lemma nra_eval_map_correct : forall e l1 l2,
+        (forall d1 d2 : data, nra_eval e d1 = Some d2 -> nra_sem e d1 d2) ->
+        rmap (nra_eval e) l1 = Some l2 ->
+        nra_sem_map e l1 l2.
+      Proof.
+        intros.
+        revert l2 H0.
+        induction l1; simpl in *; intros.
+        - inversion H0; econstructor.
+        - case_eq (nra_eval e a); intros; rewrite H1 in *; [|congruence].
+          unfold lift in H0.
+          case_eq (rmap (nra_eval e) l1); intros; rewrite H2 in *; [|congruence].
+          specialize (IHl1 l eq_refl).
+          inversion H0.
+          econstructor; eauto.
+      Qed.
 
-    (* evaluation preserves normalization *)
-    Lemma nra_eval_normalized {op:nra} {d:data} {o} :
-      Forall (fun x => data_normalized h (snd x)) constant_env ->
-      nra_eval op d = Some o ->
-      data_normalized h d ->
-      data_normalized h o.
-    Proof.
-      intro HconstNorm.
-      revert d o.
-      induction op; simpl.
-      - inversion 1; subst; trivial.
-      - inversion 1; subst; intros.
-        apply normalize_normalizes.
-      - intros.
-        specialize (IHop1 d).
-        specialize (IHop2 d).
-        destruct (nra_eval op1 d); simpl in *; try discriminate.
-        destruct (nra_eval op2 d); simpl in *; try discriminate.
-        apply (binary_op_eval_normalized h) in H; eauto.
-      - intros.
-        specialize (IHop d).
-        destruct (nra_eval op d); simpl in *; try discriminate.
-        apply unary_op_eval_normalized in H; eauto.
-      - intros;
-          specialize (IHop2 d);
-          destruct (nra_eval op2 d); simpl in *; try discriminate;
-            specialize (IHop2 _ (eq_refl _) H0).
-        destruct d0; simpl in *; try discriminate.
-        apply some_lift in H; destruct H; subst.
-        constructor.
-        inversion IHop2; subst.
-        apply (rmap_Forall e H1); eauto.
-      - intros;
-          specialize (IHop2 d);
-          destruct (nra_eval op2 d); simpl in *; try discriminate;
-            specialize (IHop2 _ (eq_refl _) H0).
-        destruct d0; simpl in *; try discriminate.
-        apply some_lift in H; destruct H; subst.
-        constructor.
-        inversion IHop2; subst.
-        unfold rmap_concat in *.
-        apply (oflat_map_Forall e H1); intros.
-        specialize (IHop1 x0).
-        unfold oomap_concat in H.
-        match_destr_in H.
-        specialize (IHop1 _ (eq_refl _) H2).
-        unfold omap_concat in H.
-        match_destr_in H.
-        inversion IHop1; subst.
-        apply (rmap_Forall H H4); intros.
-        eapply (data_normalized_orecconcat H3); trivial.
-      -  intros;
-           specialize (IHop1 d);
-           destruct (nra_eval op1 d); simpl in *; try discriminate.
-         specialize (IHop1 _ (eq_refl _) H0).
-         destruct d0; simpl in *; try discriminate.
-         apply some_lift in H; destruct H; subst.
-         constructor.
-         inversion IHop1; subst.
-         unfold rmap_concat in *.
-         apply (oflat_map_Forall e H1); intros.
-         specialize (IHop2 d).
-         unfold oomap_concat in H.
-         match_destr_in H.
-         specialize (IHop2 _ (eq_refl _) H0).
-         unfold omap_concat in H.
-         match_destr_in H.
-         inversion IHop2; subst.
-         apply (rmap_Forall H H4); intros.
-         eapply (data_normalized_orecconcat H3); trivial.
-      - intros;
-          specialize (IHop2 d);
-          destruct (nra_eval op2 d); simpl in *; try discriminate;
-            specialize (IHop2 _ (eq_refl _) H0).
-        destruct d0; simpl in *; try discriminate.
-        apply some_lift in H; destruct H; subst.      
-        constructor.
-        inversion IHop2; subst.
-        unfold rmap_concat in *.
-        apply (lift_filter_Forall e H1).
-      - intros;
-          specialize (IHop1 d);
+          
+      Lemma nra_eval_map_product_correct : forall e l1 l2,
+        (forall d1 d2 : data, nra_eval e d1 = Some d2 -> nra_sem e d1 d2) ->
+        rmap_product (nra_eval e) l1 = Some l2 ->
+        nra_sem_map_product e l1 l2.
+      Proof.
+        intros.
+        revert l2 H0.
+        induction l1; simpl in *; intros.
+        - inversion H0; econstructor.
+        - generalize (rmap_product_cons_inv (nra_eval e) l1 a l2 H0); intros.
+          elim H1; clear H1; intros.
+          elim H1; clear H1; intros.
+          elim H1; clear H1; intros.
+          elim H2; clear H2; intros.
+          subst.
+          unfold oomap_concat in H1.
+          case_eq (nra_eval e a); intros; rewrite H3 in *; [|congruence].
+          case_eq d; intros; rewrite H4 in H1; try congruence.
+          subst.
+          specialize (H a (dcoll l) H3).
+          rewrite omap_concat_correct_and_complete in H1.
+          apply (sem_NRAMapProduct_cons e a l1 x0 l x).
+          + assumption.
+          + assumption.
+          + apply IHl1; assumption.
+      Qed.
+
+      Lemma nra_eval_select_correct e l1 l2 :
+        (forall d1 d2 : data, nra_eval e d1 = Some d2 -> nra_sem e d1 d2) ->
+        lift_filter
+          (fun d1 : data =>
+             match nra_eval e d1 with
+             | Some dunit => None
+             | Some (dnat _) => None
+             | Some (dbool b) => Some b
+             | Some (dstring _) => None
+             | Some (dcoll _) => None
+             | Some (drec _) => None
+             | Some (dleft _) => None
+             | Some (dright _) => None
+             | Some (dbrand _ _) => None
+             | Some (dforeign _) => None
+             | None => None
+             end) l1 = Some l2 ->
+        nra_sem_select e l1 l2.
+      Proof.
+        intro.
+        revert l2; induction l1; simpl; intros.
+        - inversion H0. econstructor.
+        - case_eq (nra_eval e a); intros; rewrite H1 in *; simpl in *.
+          destruct d; simpl in *; try congruence.
+          case_eq
+            (lift_filter
+               (fun d1 : data =>
+                  match nra_eval e d1 with
+                  | Some dunit => None
+                  | Some (dnat _) => None
+                  | Some (dbool b) => Some b
+                  | Some (dstring _) => None
+                  | Some (dcoll _) => None
+                  | Some (drec _) => None
+                  | Some (dleft _) => None
+                  | Some (dright _) => None
+                  | Some (dbrand _ _) => None
+                  | Some (dforeign _) => None
+                  | None => None
+                  end) l1);
+            intros; rewrite H2 in *; clear H2; [|congruence].
+          specialize (IHl1 l eq_refl).
+          destruct b; simpl in *;
+            simpl in *; inversion H0; clear H0; subst.
+          + econstructor; eauto.
+          + econstructor; eauto.
+          + congruence.
+      Qed.
+
+      Lemma nra_eval_correct : forall e d1 d2,
+          nra_eval e d1 = Some d2 ->
+          nra_sem e d1 d2.
+      Proof.
+        induction e; simpl; intros.
+        - econstructor; eauto.
+        - inversion H; econstructor; eauto.
+        - inversion H; econstructor; eauto.
+        - unfold olift2 in H.
+          case_eq (nra_eval e1 d1); intros; rewrite H0 in *; [|congruence].
+          case_eq (nra_eval e2 d1); intros; rewrite H1 in *; [|congruence].
+          specialize (IHe1 d1 d H0); specialize (IHe2 d1 d0 H1);
+            econstructor; eauto.
+        - unfold olift in H.
+          case_eq (nra_eval e d1); intros; rewrite H0 in *; [|congruence].
+          specialize (IHe d1 d H0); econstructor; eauto.
+        - unfold olift in H.
+          case_eq (nra_eval e2 d1); intros; rewrite H0 in *; [|congruence].
+          unfold lift_oncoll in H.
+          destruct d; simpl in H; try congruence.
+          unfold lift in H.
+          case_eq (rmap (nra_eval e1) l); intros; rewrite H1 in *; [|congruence].
+          inversion H; subst; clear H.
+          econstructor; eauto.
+          apply nra_eval_map_correct; auto.
+        - unfold olift in H.
+          case_eq (nra_eval e2 d1); intros; rewrite H0 in *; [|congruence].
+          unfold lift_oncoll in H.
+          destruct d; simpl in H; try congruence.
+          unfold lift in H.
+          case_eq (rmap_product (nra_eval e1) l); intros; rewrite H1 in *; [|congruence].
+          inversion H; subst; clear H.
+          econstructor; eauto.
+          apply nra_eval_map_product_correct; auto.
+        - unfold olift2 in H.
+          (*
+          case_eq (nra_eval e1 d1); intros; rewrite H0 in *; [|congruence].
+          case_eq (nra_eval e2 d1); intros; rewrite H1 in *; [|congruence].
+          unfold lift_ondcoll2 in H.
+          destruct d; try congruence.
+          destruct d0; try congruence.
+          unfold lift in H.
+          case_eq (rproduct l l0); intros; rewrite H2 in *; [|congruence].
+          inversion H; subst; clear H.
+          econstructor; eauto.
+          rewrite <- rproduct_correct_and_complete. assumption.
+           *)
+          admit.
+        - unfold olift in H.
+          case_eq (nra_eval e2 d1); intros; rewrite H0 in *; [|congruence].
+          unfold lift_oncoll in H.
+          destruct d; simpl in H; try congruence.
+          unfold lift in H.
+          specialize (IHe2 d1 (dcoll l) H0).
+          case_eq
+            (lift_filter
+               (fun d1 : data =>
+                  match nra_eval e1 d1 with
+                  | Some dunit => None
+                  | Some (dnat _) => None
+                  | Some (dbool b) => Some b
+                  | Some (dstring _) => None
+                  | Some (dcoll _) => None
+                  | Some (drec _) => None
+                  | Some (dleft _) => None
+                  | Some (dright _) => None
+                  | Some (dbrand _ _) => None
+                  | Some (dforeign _) => None
+                  | None => None
+                  end) l); intros; rewrite H1 in *; [|congruence].
+          inversion H; clear H; subst.
+          econstructor; eauto.
+          apply nra_eval_select_correct; auto.
+        - unfold olift in H.
+          case_eq (nra_eval e1 d1); intros; rewrite H0 in *; [|congruence].
+          elim (data_eq_dec d (dcoll nil)); intros.
+          subst.
+          + econstructor; eauto.
+          + destruct d; inversion H; subst; auto;
+              eapply sem_NRADefault_not_empty; auto;
+                destruct l; auto; inversion H; subst; auto.
+            congruence.
+        - destruct d1; try congruence.
+          econstructor; apply IHe1; auto.
+          econstructor; apply IHe2; auto.
+        - case_eq (nra_eval e1 d1); intros; rewrite H0 in *; [|congruence].
+          destruct d; intros; try congruence.
+         + destruct d; intros; try congruence.
+            case_eq (nra_eval e2 d1); intros; rewrite H1 in *; [|congruence].
+            destruct d; intros; try congruence.
+            inversion H; subst; clear H; intros.
+            econstructor; eauto.
+          + destruct d; intros; try congruence.
+            case_eq (nra_eval e2 d1); intros; rewrite H1 in *; [|congruence].
+            destruct d; intros; try congruence.
+            inversion H; subst; clear H; intros.
+            econstructor; eauto.
+        - unfold olift in H.
+          case_eq (nra_eval e2 d1); intros; rewrite H0 in *; [|congruence].
+          econstructor; eauto.
+      Admitted.
+ 
+    End EvalCorrect.
+
+    Section EvalNormalized.
+      Lemma data_normalized_orecconcat {x y z}:
+        orecconcat x y = Some z ->
+        data_normalized h x -> data_normalized h y ->
+        data_normalized h z.
+      Proof.
+        destruct x; simpl; try discriminate.
+        destruct y; simpl; try discriminate.
+        inversion 1; subst.
+        apply data_normalized_rec_concat_sort; trivial.
+      Qed.
+
+      (* evaluation preserves normalization *)
+      Lemma nra_eval_normalized {op:nra} {d:data} {o} :
+        Forall (fun x => data_normalized h (snd x)) constant_env ->
+        nra_eval op d = Some o ->
+        data_normalized h d ->
+        data_normalized h o.
+      Proof.
+        intro HconstNorm.
+        revert d o.
+        induction op; simpl.
+        - intros.
+          unfold edot in H.
+          apply assoc_lookupr_in in H.
+          rewrite Forall_forall in HconstNorm.
+          specialize (HconstNorm (s,o)); simpl in *.
+          auto.
+        - inversion 1; subst; trivial.
+        - inversion 1; subst; intros.
+          apply normalize_normalizes.
+        - intros.
+          specialize (IHop1 d).
+          specialize (IHop2 d).
           destruct (nra_eval op1 d); simpl in *; try discriminate.
-        specialize (IHop1 _ (eq_refl _) H0).
-        destruct d0; simpl in *; try solve [inversion H; subst; trivial].
-        destruct l; simpl; eauto 3.
-        inversion H; subst; trivial.
-      - intros.
-        destruct d; try discriminate; inversion H0; subst; eauto.
-      - intros.
-        specialize (IHop1 d).
-        specialize (IHop2 d).
-        destruct (nra_eval op1 d); simpl in *; try discriminate.
-        destruct (nra_eval op2 d); simpl in *; try discriminate.
-        specialize (IHop1 _ (eq_refl _) H0).
-        specialize (IHop2 _ (eq_refl _) H0).
-        destruct d0; try discriminate.
-        + destruct d0; try discriminate.
-          destruct d1; try discriminate.
-          inversion IHop1; subst.
-          inversion H; subst.
+          destruct (nra_eval op2 d); simpl in *; try discriminate.
+          apply (binary_op_eval_normalized h) in H; eauto.
+        - intros.
+          specialize (IHop d).
+          destruct (nra_eval op d); simpl in *; try discriminate.
+          apply unary_op_eval_normalized in H; eauto.
+        - intros;
+            specialize (IHop2 d);
+            destruct (nra_eval op2 d); simpl in *; try discriminate;
+              specialize (IHop2 _ (eq_refl _) H0).
+          destruct d0; simpl in *; try discriminate.
+          apply some_lift in H; destruct H; subst.
           constructor.
-          apply data_normalized_rec_concat_sort; trivial.
-        + destruct d0; try discriminate.
-          destruct d1; try discriminate.
-          inversion IHop1; subst.
-          inversion H; subst.
+          inversion IHop2; subst.
+          apply (rmap_Forall e H1); eauto.
+        - intros;
+            specialize (IHop2 d);
+            destruct (nra_eval op2 d); simpl in *; try discriminate;
+              specialize (IHop2 _ (eq_refl _) H0).
+          destruct d0; simpl in *; try discriminate.
+          apply some_lift in H; destruct H; subst.
           constructor.
-          apply data_normalized_rec_concat_sort; trivial.
-        + repeat (destruct d0; try discriminate).
-      - intros. specialize (IHop2 d).
-        destruct (nra_eval op2 d); simpl in *; try discriminate.
-        eauto.
-      - intros.
-        unfold edot in H.
-        apply assoc_lookupr_in in H.
-        rewrite Forall_forall in HconstNorm.
-        specialize (HconstNorm (s,o)); simpl in *.
-        auto.
-    Qed.
+          inversion IHop2; subst.
+          unfold rmap_product in *.
+          apply (oflat_map_Forall e H1); intros.
+          specialize (IHop1 x0).
+          unfold oomap_concat in H.
+          match_destr_in H.
+          specialize (IHop1 _ (eq_refl _) H2).
+          unfold omap_concat in H.
+          match_destr_in H.
+          inversion IHop1; subst.
+          apply (rmap_Forall H H4); intros.
+          eapply (data_normalized_orecconcat H3); trivial.
+        - intros;
+            specialize (IHop1 d);
+            destruct (nra_eval op1 d); simpl in *; try discriminate.
+          specialize (IHop1 _ (eq_refl _) H0).
+          destruct d0; simpl in *; try discriminate.
+          apply some_lift in H; destruct H; subst.
+          constructor.
+          inversion IHop1; subst.
+          unfold rmap_product in *.
+          apply (oflat_map_Forall e H1); intros.
+          specialize (IHop2 d).
+          unfold oomap_concat in H.
+          match_destr_in H.
+          specialize (IHop2 _ (eq_refl _) H0).
+          unfold omap_concat in H.
+          match_destr_in H.
+          inversion IHop2; subst.
+          apply (rmap_Forall H H4); intros.
+          eapply (data_normalized_orecconcat H3); trivial.
+        - intros;
+          specialize (IHop2 d);
+          destruct (nra_eval op2 d); simpl in *; try discriminate;
+            specialize (IHop2 _ (eq_refl _) H0).
+          destruct d0; simpl in *; try discriminate.
+          apply some_lift in H; destruct H; subst.      
+          constructor.
+          inversion IHop2; subst.
+          unfold rmap_product in *.
+          apply (lift_filter_Forall e H1).
+        - intros;
+            specialize (IHop1 d);
+            destruct (nra_eval op1 d); simpl in *; try discriminate.
+          specialize (IHop1 _ (eq_refl _) H0).
+          destruct d0; simpl in *; try solve [inversion H; subst; trivial].
+          destruct l; simpl; eauto 3.
+          inversion H; subst; trivial.
+        - intros.
+          destruct d; try discriminate; inversion H0; subst; eauto.
+        - intros.
+          specialize (IHop1 d).
+          specialize (IHop2 d).
+          destruct (nra_eval op1 d); simpl in *; try discriminate.
+          destruct (nra_eval op2 d); simpl in *; try discriminate.
+          specialize (IHop1 _ (eq_refl _) H0).
+          specialize (IHop2 _ (eq_refl _) H0).
+          destruct d0; try discriminate.
+          + destruct d0; try discriminate.
+            destruct d1; try discriminate.
+            inversion IHop1; subst.
+            inversion H; subst.
+            constructor.
+            apply data_normalized_rec_concat_sort; trivial.
+          + destruct d0; try discriminate.
+            destruct d1; try discriminate.
+            inversion IHop1; subst.
+            inversion H; subst.
+            constructor.
+            apply data_normalized_rec_concat_sort; trivial.
+          + repeat (destruct d0; try discriminate).
+        - intros. specialize (IHop2 d).
+          destruct (nra_eval op2 d); simpl in *; try discriminate.
+          eauto.
+      Qed.
+    End EvalNormalized.
   End Semantics.
   
   Section Top.
+    Context (h:list(string*string)).
     Definition nra_eval_top (q:nra) (cenv:bindings) : option data :=
-      nra_eval (rec_sort cenv) q dunit.
+      nra_eval h (rec_sort cenv) q dunit.
   End Top.
 
   Section FreeVars.
     Fixpoint nra_free_variables (q:nra) : list string :=
       match q with
-      | AID => nil
-      | AConst _ => nil
-      | ABinop _ q1 q2 =>
+      | NRAGetConstant s => s :: nil
+      | NRAID => nil
+      | NRAConst _ => nil
+      | NRABinop _ q1 q2 =>
         app (nra_free_variables q1) (nra_free_variables q2)
-      | AUnop _ q1 =>
+      | NRAUnop _ q1 =>
         (nra_free_variables q1)
-      | AMap q1 q2 =>
+      | NRAMap q1 q2 =>
         app (nra_free_variables q1) (nra_free_variables q2)
-      | AMapConcat q1 q2 =>
+      | NRAMapProduct q1 q2 =>
         app (nra_free_variables q1) (nra_free_variables q2)
-      | AProduct q1 q2 =>
+      | NRAProduct q1 q2 =>
         app (nra_free_variables q1) (nra_free_variables q2)
-      | ASelect q1 q2 =>
+      | NRASelect q1 q2 =>
         app (nra_free_variables q1) (nra_free_variables q2)
-      | ADefault q1 q2 =>
+      | NRADefault q1 q2 =>
         app (nra_free_variables q1) (nra_free_variables q2)
-      | AEither ql qr =>
+      | NRAEither ql qr =>
         app (nra_free_variables ql) (nra_free_variables qr)
-      | AEitherConcat q1 q2 =>
+      | NRAEitherConcat q1 q2 =>
         app (nra_free_variables q1) (nra_free_variables q2)
-      | AApp q1 q2 =>
+      | NRAApp q1 q2 =>
         app (nra_free_variables q1) (nra_free_variables q2)
-      | AGetConstant s => s :: nil
     end.
   End FreeVars.
 
@@ -305,60 +791,59 @@ Notation "h ⊢ Op @ₐ x ⊣ c" := (nra_eval h c Op x) (at level 10). (* \vdash
 (* begin hide *)
 Delimit Scope nra_scope with nra.
 
-Notation "'ID'" := (AID)  (at level 50) : nra_scope.
-Notation "CGET⟨ s ⟩" := (AGetConstant s) (at level 50) : nra_core_scope.
+Notation "'ID'" := (NRAID)  (at level 50) : nra_scope.
+Notation "TABLE⟨ s ⟩" := (NRAGetConstant s) (at level 50) : nra_core_scope.
+Notation "‵‵ c" := (NRAConst (dconst c))  (at level 0) : nra_scope.                           (* ‵ = \backprime *)
+Notation "‵ c" := (NRAConst c)  (at level 0) : nra_scope.                                     (* ‵ = \backprime *)
+Notation "‵{||}" := (NRAConst (dcoll nil))  (at level 0) : nra_scope.                         (* ‵ = \backprime *)
+Notation "‵[||]" := (NRAConst (drec nil)) (at level 50) : nra_scope.                          (* ‵ = \backprime *)
 
-Notation "‵‵ c" := (AConst (dconst c))  (at level 0) : nra_scope.                           (* ‵ = \backprime *)
-Notation "‵ c" := (AConst c)  (at level 0) : nra_scope.                                     (* ‵ = \backprime *)
-Notation "‵{||}" := (AConst (dcoll nil))  (at level 0) : nra_scope.                         (* ‵ = \backprime *)
-Notation "‵[||]" := (AConst (drec nil)) (at level 50) : nra_scope.                          (* ‵ = \backprime *)
+Notation "r1 ∧ r2" := (NRABinop OpAnd r1 r2) (right associativity, at level 65): nra_scope.    (* ∧ = \wedge *)
+Notation "r1 ∨ r2" := (NRABinop OpOr r1 r2) (right associativity, at level 70): nra_scope.     (* ∨ = \vee *)
+Notation "r1 ≐ r2" := (NRABinop OpEqual r1 r2) (right associativity, at level 70): nra_scope.     (* ≐ = \doteq *)
+Notation "r1 ≤ r2" := (NRABinop OpLt r1 r2) (no associativity, at level 70): nra_scope.     (* ≤ = \leq *)
+Notation "r1 ⋃ r2" := (NRABinop OpBagUnion r1 r2) (right associativity, at level 70): nra_scope.  (* ⋃ = \bigcup *)
+Notation "r1 − r2" := (NRABinop OpBagDiff r1 r2) (right associativity, at level 70): nra_scope.  (* − = \minus *)
+Notation "r1 ⋂min r2" := (NRABinop OpBagMin r1 r2) (right associativity, at level 70): nra_scope. (* ♯ = \sharp *)
+Notation "r1 ⋃max r2" := (NRABinop OpBagMax r1 r2) (right associativity, at level 70): nra_scope. (* ♯ = \sharp *)
+Notation "p ⊕ r"   := ((NRABinop OpRecConcat) p r) (at level 70) : nra_scope.                     (* ⊕ = \oplus *)
+Notation "p ⊗ r"   := ((NRABinop OpRecMerge) p r) (at level 70) : nra_scope.                (* ⊗ = \otimes *)
 
-Notation "r1 ∧ r2" := (ABinop OpAnd r1 r2) (right associativity, at level 65): nra_scope.    (* ∧ = \wedge *)
-Notation "r1 ∨ r2" := (ABinop OpOr r1 r2) (right associativity, at level 70): nra_scope.     (* ∨ = \vee *)
-Notation "r1 ≐ r2" := (ABinop OpEqual r1 r2) (right associativity, at level 70): nra_scope.     (* ≐ = \doteq *)
-Notation "r1 ≤ r2" := (ABinop OpLt r1 r2) (no associativity, at level 70): nra_scope.     (* ≤ = \leq *)
-Notation "r1 ⋃ r2" := (ABinop OpBagUnion r1 r2) (right associativity, at level 70): nra_scope.  (* ⋃ = \bigcup *)
-Notation "r1 − r2" := (ABinop OpBagDiff r1 r2) (right associativity, at level 70): nra_scope.  (* − = \minus *)
-Notation "r1 ⋂min r2" := (ABinop OpBagMin r1 r2) (right associativity, at level 70): nra_scope. (* ♯ = \sharp *)
-Notation "r1 ⋃max r2" := (ABinop OpBagMax r1 r2) (right associativity, at level 70): nra_scope. (* ♯ = \sharp *)
-Notation "p ⊕ r"   := ((ABinop OpRecConcat) p r) (at level 70) : nra_scope.                     (* ⊕ = \oplus *)
-Notation "p ⊗ r"   := ((ABinop OpRecMerge) p r) (at level 70) : nra_scope.                (* ⊗ = \otimes *)
+Notation "¬( r1 )" := (NRAUnop OpNeg r1) (right associativity, at level 70): nra_scope.        (* ¬ = \neg *)
+Notation "ε( r1 )" := (NRAUnop OpDistinct r1) (right associativity, at level 70): nra_scope.   (* ε = \epsilon *)
+Notation "♯count( r1 )" := (NRAUnop OpCount r1) (right associativity, at level 70): nra_scope. (* ♯ = \sharp *)
+Notation "♯flatten( d )" := (NRAUnop OpFlatten d) (at level 50) : nra_scope.                   (* ♯ = \sharp *)
+Notation "‵{| d |}" := ((NRAUnop OpBag) d)  (at level 50) : nra_scope.                        (* ‵ = \backprime *)
+Notation "‵[| ( s , r ) |]" := ((NRAUnop (OpRec s)) r) (at level 50) : nra_scope.              (* ‵ = \backprime *)
+Notation "¬π[ s1 ]( r )" := ((NRAUnop (OpRecRemove s1)) r) (at level 50) : nra_scope.          (* ¬ = \neg and π = \pi *)
+Notation "π[ s1 ]( r )" := ((NRAUnop (OpRecProject s1)) r) (at level 50) : nra_scope.          (* π = \pi *)
+Notation "p · r" := ((NRAUnop (OpDot r)) p) (left associativity, at level 40): nra_scope.      (* · = \cdot *)
 
-Notation "¬( r1 )" := (AUnop OpNeg r1) (right associativity, at level 70): nra_scope.        (* ¬ = \neg *)
-Notation "ε( r1 )" := (AUnop OpDistinct r1) (right associativity, at level 70): nra_scope.   (* ε = \epsilon *)
-Notation "♯count( r1 )" := (AUnop OpCount r1) (right associativity, at level 70): nra_scope. (* ♯ = \sharp *)
-Notation "♯flatten( d )" := (AUnop OpFlatten d) (at level 50) : nra_scope.                   (* ♯ = \sharp *)
-Notation "‵{| d |}" := ((AUnop OpBag) d)  (at level 50) : nra_scope.                        (* ‵ = \backprime *)
-Notation "‵[| ( s , r ) |]" := ((AUnop (OpRec s)) r) (at level 50) : nra_scope.              (* ‵ = \backprime *)
-Notation "¬π[ s1 ]( r )" := ((AUnop (OpRecRemove s1)) r) (at level 50) : nra_scope.          (* ¬ = \neg and π = \pi *)
-Notation "π[ s1 ]( r )" := ((AUnop (OpRecProject s1)) r) (at level 50) : nra_scope.          (* π = \pi *)
-Notation "p · r" := ((AUnop (OpDot r)) p) (left associativity, at level 40): nra_scope.      (* · = \cdot *)
-
-Notation "χ⟨ p ⟩( r )" := (AMap p r) (at level 70) : nra_scope.                              (* χ = \chi *)
-Notation "⋈ᵈ⟨ e2 ⟩( e1 )" := (AMapConcat e2 e1) (at level 70) : nra_scope.                   (* ⟨ ... ⟩ = \rangle ...  \langle *)
-Notation "r1 × r2" := (AProduct r1 r2) (right associativity, at level 70): nra_scope.       (* × = \times *)
-Notation "σ⟨ p ⟩( r )" := (ASelect p r) (at level 70) : nra_scope.                           (* σ = \sigma *)
-Notation "r1 ∥ r2" := (ADefault r1 r2) (right associativity, at level 70): nra_scope.       (* ∥ = \parallel *)
-Notation "r1 ◯ r2" := (AApp r1 r2) (right associativity, at level 60): nra_scope.           (* ◯ = \bigcirc *)
+Notation "χ⟨ p ⟩( r )" := (NRAMap p r) (at level 70) : nra_scope.                              (* χ = \chi *)
+Notation "⋈ᵈ⟨ e2 ⟩( e1 )" := (NRAMapProduct e2 e1) (at level 70) : nra_scope.                   (* ⟨ ... ⟩ = \rangle ...  \langle *)
+Notation "r1 × r2" := (NRAProduct r1 r2) (right associativity, at level 70): nra_scope.       (* × = \times *)
+Notation "σ⟨ p ⟩( r )" := (NRASelect p r) (at level 70) : nra_scope.                           (* σ = \sigma *)
+Notation "r1 ∥ r2" := (NRADefault r1 r2) (right associativity, at level 70): nra_scope.       (* ∥ = \parallel *)
+Notation "r1 ◯ r2" := (NRAApp r1 r2) (right associativity, at level 60): nra_scope.           (* ◯ = \bigcirc *)
 
 Hint Resolve nra_eval_normalized.
 
 Local Open Scope string_scope.
 Tactic Notation "nra_cases" tactic(first) ident(c) :=
   first;
-  [ Case_aux c "AID"
-  | Case_aux c "AConst"
-  | Case_aux c "ABinop"
-  | Case_aux c "AUnop"
-  | Case_aux c "AMap"
-  | Case_aux c "AMapConcat"
-  | Case_aux c "AProduct"
-  | Case_aux c "ASelect"
-  | Case_aux c "ADefault"
-  | Case_aux c "AEither"
-  | Case_aux c "AEitherConcat"
-  | Case_aux c "AApp"
-  | Case_aux c "AGetConstant" ].
+  [ Case_aux c "NRAGetConstant"
+  | Case_aux c "NRAID"
+  | Case_aux c "NRAConst"
+  | Case_aux c "NRABinop"
+  | Case_aux c "NRAUnop"
+  | Case_aux c "NRAMap"
+  | Case_aux c "NRAMapProduct"
+  | Case_aux c "NRAProduct"
+  | Case_aux c "NRASelect"
+  | Case_aux c "NRADefault"
+  | Case_aux c "NRAEither"
+  | Case_aux c "NRAEitherConcat"
+  | Case_aux c "NRAApp" ].
 
 (* end hide *)
 
